Remove warnings in extraction impls (#192)
* Remove warnings in extraction impls

* Update a bit

theories/Extraction/NbE.v
@@ -15,7 +15,7 @@ Inductive initial_env_order : ctx -> Prop :=
      initial_env_order (A :: Γ)).
 
 #[local]
-  Hint Constructors initial_env_order : mcltt.
+Hint Constructors initial_env_order : mcltt.
 
 Lemma initial_env_order_sound : forall Γ p,
     initial_env Γ p ->
@@ -25,24 +25,24 @@ Proof with (econstructor; intros; functional_initial_env_rewrite_clear; function
 Qed.
 
 #[local]
-  Hint Resolve initial_env_order_sound : mcltt.
+Hint Resolve initial_env_order_sound : mcltt.
 
 Derive Signature for initial_env_order.
 
 Section InitialEnvImpl.
 
   #[local]
-    Ltac impl_obl_tac1 :=
+  Ltac impl_obl_tac1 :=
   match goal with
   | H : initial_env_order _ |- _ => progressive_invert H
   end.
 
   #[local]
-    Ltac impl_obl_tac :=
+  Ltac impl_obl_tac :=
     repeat impl_obl_tac1; try econstructor; mauto.
 
-  #[tactic="impl_obl_tac"]
-    Equations initial_env_impl G (H : initial_env_order G) : { p | initial_env G p } by struct H :=
+  #[tactic="impl_obl_tac",derive(equations=no,eliminator=no)]
+  Equations initial_env_impl G (H : initial_env_order G) : { p | initial_env G p } by struct H :=
   | nil, H => exist _ empty_env _
   | cons A G, H =>
       let (p, Hp) := initial_env_impl G _ in
@@ -51,29 +51,40 @@ Section InitialEnvImpl.
 
 End InitialEnvImpl.
 
-
-Lemma initial_env_impl_complete' : forall G p,
-    initial_env G p ->
-    forall (H : initial_env_order G),
-      exists H', initial_env_impl G H = exist _ p H'.
-Proof.
-  induction 1;
-    pose proof eval_exp_impl_complete';
-    intros; simp initial_env_impl;
-    do 2 try complete_tac;
-    eauto.
-Qed.
-
-#[local]
-Hint Resolve initial_env_impl_complete' : mcltt.
-
+(** The definitions of [initial_env_impl] already come with soundness proofs,
+    so we only need to prove completeness. However, the completeness
+    is also obvious from the soundness of eval orders and functional
+    nature of initial_env. *)
 
 Lemma initial_env_impl_complete : forall G p,
     initial_env G p ->
     exists H H', initial_env_impl G H = exist _ p H'.
 Proof.
-  repeat unshelve mauto.
+  intros.
+  assert (Horder : initial_env_order G) by mauto.
+  exists Horder.
+  destruct (initial_env_impl G Horder).
+  functional_initial_env_rewrite_clear.
+  eexists; reflexivity.
 Qed.
+
+(** A similar approach works for nbe implementations.
+    However, as we have 2 implementations (each for [nbe] and [nbe_ty]),
+    We define a tactic to deal with both cases. *)
+
+Ltac functional_nbe_complete :=
+  lazymatch goal with
+  | |- exists (_ : ?T), _ =>
+      let Horder := fresh "Horder" in
+      assert T as Horder by mauto 3;
+      eexists Horder;
+      lazymatch goal with
+      | |- exists _, ?L = _ =>
+          destruct L;
+          functional_nbe_rewrite_clear;
+          eexists; reflexivity
+      end
+  end.
 
 Inductive nbe_order G M A : Prop :=
 | nbe_order_run :
@@ -90,8 +101,7 @@ Inductive nbe_order G M A : Prop :=
      nbe_order G M A ).
 
 #[local]
-  Hint Constructors nbe_order : mcltt.
-
+Hint Constructors nbe_order : mcltt.
 
 Lemma nbe_order_sound : forall G M A w,
     nbe G M A w ->
@@ -105,22 +115,22 @@ Proof with (econstructor; intros;
 Qed.
 
 #[local]
-  Hint Resolve nbe_order_sound : mcltt.
+Hint Resolve nbe_order_sound : mcltt.
 
 Section NbEDef.
 
   #[local]
-    Ltac impl_obl_tac1 :=
+  Ltac impl_obl_tac1 :=
   match goal with
   | H : nbe_order _ _ _ |- _ => progressive_invert H
   end.
 
   #[local]
-    Ltac impl_obl_tac :=
+  Ltac impl_obl_tac :=
     repeat impl_obl_tac1; try econstructor; mauto.
 
-  #[tactic="impl_obl_tac"]
-    Equations nbe_impl G M A (H : nbe_order G M A) : { w | nbe G M A w } by struct H :=
+  #[tactic="impl_obl_tac",derive(equations=no,eliminator=no)]
+  Equations nbe_impl G M A (H : nbe_order G M A) : { w | nbe G M A w } by struct H :=
   | G, M, A, H =>
       let (p, Hp) := initial_env_impl G _ in
       let (a, Ha) := eval_exp_impl A p _ in
@@ -128,32 +138,14 @@ Section NbEDef.
       let (w, Hw) := read_nf_impl (length G) d{{{ ⇓ a m }}} _ in
       exist _ w _.
 
-  Lemma nbe_impl_complete' : forall G M A w,
-      nbe G M A w ->
-      forall (H : nbe_order G M A),
-      exists H', nbe_impl G M A H = exist _ w H'.
-  Proof.
-    induction 1;
-      pose proof initial_env_impl_complete';
-      pose proof eval_exp_impl_complete';
-      pose proof read_nf_impl_complete';
-      intros; simp nbe_impl;
-      repeat complete_tac;
-      eauto.
-  Qed.
-
 End NbEDef.
-
-#[local]
-  Hint Resolve nbe_impl_complete' : mcltt.
 
 Lemma nbe_impl_complete : forall G M A w,
     nbe G M A w ->
-      exists H H', nbe_impl G M A H = exist _ w H'.
+    exists H H', nbe_impl G M A H = exist _ w H'.
 Proof.
-  repeat unshelve mauto.
+  intros; functional_nbe_complete.
 Qed.
-
 
 Inductive nbe_ty_order G A : Prop :=
 | nbe_ty_order_run :
@@ -167,8 +159,7 @@ Inductive nbe_ty_order G A : Prop :=
      nbe_ty_order G A ).
 
 #[local]
-  Hint Constructors nbe_ty_order : mcltt.
-
+Hint Constructors nbe_ty_order : mcltt.
 
 Lemma nbe_ty_order_sound : forall G A w,
     nbe_ty G A w ->
@@ -182,22 +173,22 @@ Proof with (econstructor; intros;
 Qed.
 
 #[local]
-  Hint Resolve nbe_ty_order_sound : mcltt.
+Hint Resolve nbe_ty_order_sound : mcltt.
 
 Section NbETyDef.
 
   #[local]
-    Ltac impl_obl_tac1 :=
+  Ltac impl_obl_tac1 :=
   match goal with
   | H : nbe_ty_order _ _ |- _ => progressive_invert H
   end.
 
   #[local]
-    Ltac impl_obl_tac :=
+  Ltac impl_obl_tac :=
     repeat impl_obl_tac1; try econstructor; mauto.
 
-  #[tactic="impl_obl_tac"]
-    Equations nbe_ty_impl G A (H : nbe_ty_order G A) : { w | nbe_ty G A w } by struct H :=
+  #[tactic="impl_obl_tac",derive(equations=no,eliminator=no)]
+  Equations nbe_ty_impl G A (H : nbe_ty_order G A) : { w | nbe_ty G A w } by struct H :=
   | G, A, H =>
       let (p, Hp) := initial_env_impl G _ in
       let (a, Ha) := eval_exp_impl A p _ in
@@ -206,26 +197,9 @@ Section NbETyDef.
 
 End NbETyDef.
 
-Lemma nbe_ty_impl_complete' : forall G A w,
-    nbe_ty G A w ->
-    forall (H : nbe_ty_order G A),
-      exists H', nbe_ty_impl G A H = exist _ w H'.
-Proof.
-  induction 1;
-    pose proof initial_env_impl_complete';
-    pose proof eval_exp_impl_complete';
-    pose proof read_typ_impl_complete';
-    intros; simp nbe_ty_impl;
-    repeat complete_tac;
-    eauto.
-Qed.
-
-#[local]
-  Hint Resolve nbe_ty_impl_complete' : mcltt.
-
 Lemma nbe_ty_impl_complete : forall G A w,
     nbe_ty G A w ->
-      exists H H', nbe_ty_impl G A H = exist _ w H'.
+    exists H H', nbe_ty_impl G A H = exist _ w H'.
 Proof.
-  repeat unshelve mauto.
+  intros; functional_nbe_complete.
 Qed.
